code/ecdsap256/Hacl.Impl.P256.PointInverse.fst
@@ -40,6 +40,26 @@ let copyH a b =
   upd b (size 2) a2;
   upd b (size 3) a3
 
+val point_inv: p: point -> result: point -> tempBuffer: lbuffer uint64 (size 88) -> Stack unit
+  (requires fun h -> live h p /\ live h tempBuffer /\ live h result /\
+    disjoint p tempBuffer /\ disjoint result tempBuffer /\
+    eq_or_disjoint p result /\
+    as_nat h (gsub p (size 8) (size 4)) < prime /\ 
+    as_nat h (gsub p (size 0) (size 4)) < prime /\ 
+    as_nat h (gsub p (size 4) (size 4)) < prime)
+  (ensures fun h0 _ h1 -> modifies (loc tempBuffer |+| loc result)  h0 h1 /\  
+    as_nat h1 (gsub result (size 8) (size 4)) < prime /\ 
+    as_nat h1 (gsub result (size 0) (size 4)) < prime /\ 
+    as_nat h1 (gsub result (size 4) (size 4)) < prime /\ (
+  
+    let x, y, z = gsub p (size 0) (size 4),  gsub p (size 4) (size 4), gsub p (size 8) (size 4) in 
+    let x3, y3, z3 = gsub result (size 0) (size 4), gsub result (size 4) (size 4), gsub result (size 8) (size 4) in 
+      
+    let xD, yD, zD = fromDomain_ (as_nat h0 x), fromDomain_ (as_nat h0 y), fromDomain_ (as_nat h0 z) in 
+    let x3D, y3D, z3D = fromDomain_ (as_nat h1 x3), fromDomain_ (as_nat h1 y3), fromDomain_ (as_nat h1 z3) in
+      
+    let xN, yN, zN = _point_inverse (xD, yD, zD) in 
+    x3D == xN /\ y3D == yN /\ z3D == zN)) 
 
 
 let point_inv p result tempBuffer = 
@@ -56,3 +76,26 @@ let point_inv p result tempBuffer =
   let h1 = ST.get() in 
   lemmaFromDomain 0;
   FStar.Math.Lemmas.small_mod 0 prime256
+
+
+friend Hacl.Impl.P256.PointAdd8
+open  Hacl.Impl.P256.Core
+open Hacl.Impl.P256.PointAdd8
+open Lib.ByteSequence 
+
+let point_inv8 result p = 
+  push_frame();
+    let tempBuffer = create (size 112) (u64 0) in 
+    let h0 = ST.get() in 
+    let pU64 = sub tempBuffer (size 0) (size 12) in 
+    let resultU64 = sub tempBuffer (size 12) (size 12) in 
+    let tB88 = sub tempBuffer (size 24) (size 88) in 
+
+    toFormPoint p pU64; 
+    pointToDomain pU64 pU64;
+    
+    point_inv pU64 resultU64 tB88;
+    
+    norm resultU64 resultU64 tB88;
+    fromFormPoint resultU64 result;
+  pop_frame()
