code/ecdsap256/Hacl.P256.fst
@@ -89,3 +89,5 @@ let point_add8 result p q = Hacl.Impl.P256.PointAdd8.point_add8 result p q
 
 
 let verifyQPrivate pubKey = Hacl.Impl.P256.ScalarMult.verifyQPrivate pubKey
+
+let point_inv8 result p = Hacl.Impl.P256.PointInverse.point_inv8 result p
