code/ecdsap256/Hacl.P256.fsti
@@ -467,8 +467,6 @@ val point_add8: result: lbuffer uint8 (size 64) -> p: lbuffer uint8 (size 64) ->
   \n Output: bool, where 0 stands for the public key to be correct with respect to SP 800-56A:  \n Verify that the public key is not the “point at infinity”, represented as O. \n Verify that the affine x and y coordinates of the point represented by the public key are in the range [0, p – 1] where p is the prime defining the finite field. \n Verify that y2 = x3 + ax + b where a and b are the coefficients of the curve equation. \n Verify that nQ = O (the point at infinity), where n is the order of the curve and Q is the public key point.
   \n The last extract is taken from : https://neilmadden.blog/2017/05/17/so-how-do-you-validate-nist-ecdh-public-keys/
   \n The check for correctness of the order was removed because the curve is prime.")]
-
-inline_for_extraction noextract
 val verifyQPrivate: 
   pubKey: lbuffer uint8 (size 64) ->
   Stack bool
@@ -478,3 +476,22 @@ val verifyQPrivate:
     let publicKeyY = nat_from_bytes_be (as_seq h1 (gsub pubKey (size 32) (size 32))) in
     let pkJ = Spec.P256.toJacobianCoordinates (publicKeyX, publicKeyY) in 
     r == not (Spec.ECDSA.verifyQValidCurvePointSpec pkJ)))
+
+
+val point_inv8: result: lbuffer uint8 (size 64) -> p: lbuffer uint8 (size 64) ->
+  Stack unit 
+  (requires fun h -> live h result /\ live h p /\ (
+    let pX = gsub p (size 0) (size 32) in 
+    let pY = gsub p (size 32) (size 32) in 
+    
+    Lib.ByteSequence.nat_from_bytes_be (as_seq h pX) < prime256 /\ 
+    Lib.ByteSequence.nat_from_bytes_be (as_seq h pY) < prime256))
+  (ensures fun h0 _ h1 -> modifies (loc result) h0 h1 /\ (
+    let open Lib.ByteSequence in 
+    let pX = nat_from_bytes_be (as_seq h0 (gsub p (size 0) (size 32))) in 
+    let pY = nat_from_bytes_be (as_seq h0 (gsub p (size 32) (size 32))) in
+    let pK = Spec.P256.toJacobianCoordinates (pX, pY) in 
+    let resultX, resultY, _ = Spec.P256._norm (Spec.P256._point_inverse pK) in 
+    
+    as_seq h1 (gsub result (size 0) (size 32)) == nat_to_bytes_be 32 resultX /\
+    as_seq h1 (gsub result (size 32) (size 32)) == nat_to_bytes_be 32 resultY))
